InheritanceNoCR.v
@@ -1,7 +1,7 @@
 From Elo Require Import Core.
 
 From Elo Require Import NoCR.
-From Elo Require Import ValidBlocks.
+From Elo Require Import ValidTerm.
 
 Local Lemma nocr_inheritance_subst : forall x Tx t tx ad,
   no_cr ad tx ->
@@ -16,11 +16,11 @@ Qed.
 (* ------------------------------------------------------------------------- *)
 
 Local Ltac solve_nocr_inheritance :=
-  intros; ind_tstep; repeat invc_vb; try invc_nocr;
-  auto using nocr_from_value, nocr_inheritance_subst, no_cr.
+  intros; ind_tstep; repeat invc_vtm; try invc_nocr;
+  eauto using nocr_from_value, nocr_inheritance_subst, no_cr.
 
-Lemma nocr_inheritance_none : forall ad t1 t2,
-  valid_blocks t1 ->
+Lemma nocr_inheritance_none : forall ad m t1 t2,
+  valid_term m t1 ->
   (* --- *)
   no_cr ad t2 ->
   t1 --[e_none]--> t2 ->
@@ -33,8 +33,8 @@ Lemma nocr_inheritance_alloc : forall ad t1 t2 ad' T',
   no_cr ad t1.
 Proof. solve_nocr_inheritance. Qed.
 
-Lemma nocr_inheritance_insert : forall ad t1 t2 ad' t' T',
-  valid_blocks t1 ->
+Lemma nocr_inheritance_insert : forall ad m t1 t2 ad' t' T',
+  valid_term m t1 ->
   (* --- *)
   no_cr ad t2 ->
   t1 --[e_insert ad' t' T']--> t2 ->
@@ -47,16 +47,16 @@ Lemma nocr_inheritance_read : forall ad t1 t2 ad' t',
   no_cr ad t1.
 Proof. solve_nocr_inheritance. Qed.
 
-Lemma nocr_inheritance_write : forall ad t1 t2 ad' t',
-  valid_blocks t1 ->
+Lemma nocr_inheritance_write : forall ad m t1 t2 ad' t',
+  valid_term m t1 ->
   (* --- *)
   no_cr ad t2 ->
   t1 --[e_write ad' t']--> t2 ->
   no_cr ad t1.
 Proof. solve_nocr_inheritance. Qed.
 
-Lemma nocr_inheritance_acq : forall ad t1 t2 ad' t',
-  valid_blocks t1 ->
+Lemma nocr_inheritance_acq : forall ad m t1 t2 ad' t',
+  valid_term m t1 ->
   (* --- *)
   no_cr ad t2 ->
   t1 --[e_acq ad' t']--> t2 ->
@@ -70,8 +70,8 @@ Lemma nocr_inheritance_rel : forall ad t1 t2 ad',
   no_cr ad t1.
 Proof. solve_nocr_inheritance. Qed.
 
-Lemma nocr_inheritance_spawn : forall ad t1 t2 tid t,
-  valid_blocks t1 ->
+Lemma nocr_inheritance_spawn : forall ad m t1 t2 tid t,
+  valid_term m t1 ->
   (* --- *)
   no_cr ad t2 ->
   t1 --[e_spawn tid t]--> t2 ->
