SyntacticProperties.v
@@ -1,10 +1,10 @@
-From Elo Require Export ValidAddresses.
-From Elo Require Export HasVar.
 From Elo Require Export NoRef.
-From Elo Require Export NoWRef.
 From Elo Require Export NoInit.
 From Elo Require Export NoCR.
-From Elo Require Export ValidBlocks.
+From Elo Require Export HasVar.
+From Elo Require Export NoWRef.
+
+From Elo Require Export ValidTerm.
 From Elo Require Export InheritanceNoInit.
 From Elo Require Export InheritanceNoCR.
 From Elo Require Export OneInit.
