UniqueInits.v
@@ -2,10 +2,10 @@ From Coq Require Import Lia.
 
 From Elo Require Import Core.
 
-From Elo Require Import ValidAddresses.
 From Elo Require Import NoRef.
 From Elo Require Import NoInit.
-From Elo Require Import ValidBlocks.
+From Elo Require Import NoCR.
+From Elo Require Import ValidTerm.
 From Elo Require Import OneInit.
 From Elo Require Import NoUninitRefs.
 
@@ -47,10 +47,21 @@ Proof.
   eauto using noinit_oneinit_contradiction.
 Qed.
 
+(* preservation lemmas ----------------------------------------------------- *)
+
+Lemma ui_mem_region : forall m ths ad R,
+  unique_initializers m ths ->
+  unique_initializers m[ad.R <- R] ths.
+Proof.
+  intros * H. intros ad' ?. specialize (H ad').
+  repeat omicron; upsilon; destruct H; trivial;
+  split; repeat intro; repeat omicron; upsilon; spec; eauto.
+Qed.
+
 (* preservation ------------------------------------------------------------ *)
 
 Local Lemma ui_preservation_none : forall m ths tid t,
-  forall_threads ths valid_blocks ->
+  forall_threads ths (valid_term m) ->
   (* --- *)
   tid < #ths ->
   unique_initializers m ths ->
@@ -66,7 +77,7 @@ Proof.
 Qed.
 
 Local Lemma ui_preservation_alloc : forall m ths tid t T,
-  forall_threads ths (valid_addresses m) ->
+  forall_threads ths (valid_term m) ->
   (* --- *)
   tid < #ths ->
   unique_initializers m ths ->
@@ -83,22 +94,21 @@ Proof.
       split; intros; omicron;
       eauto using noinit_preservation_alloc, oneinit_preservation_alloc.
   - split; intros; upsilon; auto. exists tid. split; intros; sigma;
-    eauto using noinit_from_vad1, noinit_to_oneinit.
+    eauto using noinit_from_vtm1, noinit_to_oneinit.
   - lia.
 Qed.
 
 Local Lemma ui_preservation_insert : forall m ths tid t ad' t' T',
-  forall_threads ths (valid_addresses m) ->
-  forall_threads ths valid_blocks ->
+  forall_threads ths (valid_term m) ->
   (* --- *)
   tid < #ths ->
   unique_initializers m ths ->
   ths[tid] --[e_insert ad' t' T']--> t ->
   unique_initializers m[ad'.t <- t'] ths[tid <- t].
 Proof.
-  intros until 2.
+  intros until 1.
   intros ? Hui ? ad Had. sigma. specialize (Hui ad Had) as [Hfall Hfone].
-  assert (ad < #m) by eauto using vad_insert_address.
+  assert (ad < #m) by eauto using vtm_insert_address.
   opt_dec (m[ad].t); spec; split; intros.
   - specialize Hfone as [tid'' [? ?]].
     intros tid'. repeat omicron; nat_eq_dec tid'' tid';
@@ -131,8 +141,7 @@ Proof.
 Qed.
 
 Local Lemma ui_preservation_write : forall m ths tid t ad te,
-  forall_threads ths (valid_addresses m) ->
-  forall_threads ths valid_blocks ->
+  forall_threads ths (valid_term m) ->
   no_uninitialized_references m ths ->
   (* --- *)
   tid < #ths ->
@@ -140,9 +149,9 @@ Local Lemma ui_preservation_write : forall m ths tid t ad te,
   ths[tid] --[e_write ad te]--> t ->
   unique_initializers m[ad.t <- te] ths[tid <- t].
 Proof.
-  intros until 2. intros Hnur.
+  intros until 1. intros Hnur.
   intros ? Hui ? ad' Had'. sigma. specialize (Hui ad' Had') as [Hfall Hfone].
-  assert (ad < #m) by eauto using vad_write_address.
+  assert (ad < #m) by eauto using vtm_write_address.
   split; intros; repeat omicron; try discriminate; try spec.
   - destruct (_opt_dec m[ad'].t) as [Hmad' | Hmad']; spec.
     + destruct (Hnur ad' Hmad').
@@ -186,7 +195,7 @@ Proof.
 Qed.
 
 Local Lemma ui_preservation_spawn : forall m ths tid t te,
-  forall_threads ths valid_blocks ->
+  forall_threads ths (valid_term m) ->
   (* --- *)
   tid < #ths ->
   unique_initializers m ths ->
@@ -205,24 +214,69 @@ Proof.
     + eauto using noinit_spawn_term.
 Qed.
 
-Theorem ui_preservation : forall m1 m2 ths1 ths2 tid e,
-  forall_memory m1 no_inits ->
-  forall_program m1 ths1 (valid_addresses m1) ->
-  forall_program m1 ths1 valid_blocks ->
-  no_uninitialized_references m1 ths1 ->
+(* ------------------------------------------------------------------------- *)
+
+Theorem ui_preservation_cstep : forall m1 m2 ths1 ths2 tid e,
+  forall_memory  m1 value                ->
+  forall_program m1 ths1 (valid_term m1) ->
+  no_uninitialized_references m1 ths1    ->
   (* --- *)
   unique_initializers m1 ths1 ->
   m1 / ths1 ~~[tid, e]~~> m2 / ths2 ->
   unique_initializers m2 ths2.
 Proof.
-  intros * ? [? ?] [? ?] ? **. invc_cstep; try invc_mstep.
+  intros * ? [? ?] **. invc_cstep; try invc_mstep.
   - eauto using ui_preservation_none.
   - eauto using ui_preservation_alloc.
   - eauto using ui_preservation_insert.
-  - eauto using ui_preservation_read.
+  - eauto using noinits_from_value, ui_preservation_read.
   - eauto using ui_preservation_write.
-  - eauto using ui_preservation_acq.
+  - eauto using noinits_from_value, ui_preservation_acq.
   - eauto using ui_preservation_rel.
   - eauto using ui_preservation_spawn.
+Qed.
+
+Theorem ui_preservation_rstep : forall m1 m2 ths1 ths2 tid e,
+  forall_memory  m1 value                ->
+  forall_program m1 ths1 (valid_term m1) ->
+  no_uninitialized_references m1 ths1    ->
+  (* --- *)
+  unique_initializers m1 ths1 ->
+  m1 / ths1 ~~~[tid, e]~~> m2 / ths2 ->
+  unique_initializers m2 ths2.
+Proof.
+  intros. invc_ostep; eauto using ui_preservation_cstep.
+  match goal with _ : _ / _ ~~[_, _]~~> ?m / ?ths |- _ =>
+    assert (unique_initializers m ths)
+  end;
+  eauto using ui_preservation_cstep, ui_mem_region.
+Qed.
+
+Theorem ui_preservation_ustep : forall m1 m2 ths1 ths2 tc,
+  forall_memory  m1 value                ->
+  forall_program m1 ths1 (valid_term m1) ->
+  no_uninitialized_references m1 ths1    ->
+  (* --- *)
+  unique_initializers m1 ths1 ->
+  m1 / ths1 ~~[tc]~~>* m2 / ths2 ->
+  unique_initializers m2 ths2.
+Proof.
+  intros. ind_ustep;
+  eauto 6 using ui_preservation_rstep,
+    value_preservation_ustep,
+    vtm_preservation_ustep,
+    nur_preservation_ustep.
+Qed.
+
+Theorem ui_preservation_base : forall t,
+  no_refs  t ->
+  no_inits t ->
+  no_crs   t ->
+  (* --- *)
+  unique_initializers base_m (base_t t).
+Proof.
+  unfold base_m, base_t. intros ** ? ?. split; intros Hnil.
+  - intros ad'. simpl in Hnil. destruct ad; upsilon; auto.
+  - simpl in Hnil. destruct ad; upsilon; simpl in *; lia.
 Qed.
 
