ValidTerm.v
@@ -1,0 +1,432 @@
+From Coq Require Import Lia.
+
+From Elo Require Import Core.
+
+From Elo Require Import NoRef.
+From Elo Require Import NoInit.
+From Elo Require Import NoCR.
+
+(* ------------------------------------------------------------------------- *)
+(* valid-term                                                                *)
+(* ------------------------------------------------------------------------- *)
+
+(*
+  Enforces that:
+  - addresses are within the bounds of the memory.
+  - static blocks do not contain <init>s and <cr>s.
+*)
+Inductive valid_term (m : mem) : tm -> Prop :=
+  | vtm_unit  :                 valid_term m <{unit         }> 
+  | vtm_nat   : forall n,       valid_term m <{nat n        }>
+  | vtm_var   : forall x,       valid_term m <{var x        }>
+  | vtm_fun   : forall x Tx t,  no_inits t      ->
+                                no_crs   t      ->
+                                valid_term m t  ->
+                                valid_term m <{fn x Tx t    }>
+  | vtm_call  : forall t1 t2,   valid_term m t1 ->
+                                valid_term m t2 ->
+                                valid_term m <{call t1 t2   }> 
+  | vtm_ref   : forall ad T,    ad < #m         ->
+                                valid_term m <{&ad : T      }>
+  | vtm_init  : forall ad t T,  ad < #m         ->
+                                valid_term m t  ->
+                                valid_term m <{init ad t : T}> 
+  | vtm_new   : forall T t,     no_inits t      ->
+                                no_crs   t      ->
+                                valid_term m t  ->
+                                valid_term m <{new t : T    }>
+  | vtm_load  : forall t,       valid_term m t  ->
+                                valid_term m <{*t           }> 
+  | vtm_asg   : forall t1 t2,   valid_term m t1 ->
+                                valid_term m t2 ->
+                                valid_term m <{t1 := t2     }> 
+  | vtm_acq   : forall t1 x t2, no_inits t2     ->
+                                no_crs   t2     ->
+                                valid_term m t1 ->
+                                valid_term m t2 ->
+                                valid_term m <{acq t1 x t2  }>
+  | vtm_cr    : forall ad t,    ad < #m         ->
+                                valid_term m t  ->
+                                valid_term m <{cr ad t      }>
+  | vtm_spawn : forall t,       no_inits t      ->
+                                no_crs   t      ->
+                                valid_term m t  ->
+                                valid_term m <{spawn t      }>
+  .
+
+(* inversion --------------------------------------------------------------- *)
+
+Local Ltac _vtm tt :=
+  match goal with
+  | H : valid_term _ <{unit        }> |- _ => clear H
+  | H : valid_term _ <{nat _       }> |- _ => clear H
+  | H : valid_term _ <{var _       }> |- _ => clear H
+  | H : valid_term _ <{fn _ _ _    }> |- _ => tt H
+  | H : valid_term _ <{call _ _    }> |- _ => tt H
+  | H : valid_term _ <{& _ : _     }> |- _ => tt H
+  | H : valid_term _ <{new _ : _   }> |- _ => tt H
+  | H : valid_term _ <{init _ _ : _}> |- _ => tt H
+  | H : valid_term _ <{* _         }> |- _ => tt H
+  | H : valid_term _ <{_ := _      }> |- _ => tt H
+  | H : valid_term _ <{acq _ _ _   }> |- _ => tt H
+  | H : valid_term _ <{cr _ _      }> |- _ => tt H
+  | H : valid_term _ <{spawn _     }> |- _ => tt H
+  end.
+
+Ltac inv_vtm  := _vtm inv.
+Ltac invc_vtm := _vtm invc.
+
+(* lemmas ------------------------------------------------------------------ *)
+
+Lemma vtm_from_base : forall m t,
+  no_refs  t ->
+  no_inits t ->
+  no_crs   t ->
+  valid_term m t.
+Proof.
+  intros. induction t; invc_norefs; invc_noinits; invc_nocrs;
+  eauto using valid_term.
+Qed.
+
+Lemma vtm_insert_term : forall m t1 t2 ad t T,
+  valid_term m t1 ->
+  t1 --[e_insert ad t T]--> t2 ->
+  valid_term m t.
+Proof.
+  intros. ind_tstep; invc_vtm; auto.
+Qed.
+
+Lemma vtm_write_term : forall m t1 t2 ad t,
+  valid_term m t1 ->
+  t1 --[e_write ad t]--> t2 ->
+  valid_term m t.
+Proof.
+  intros. ind_tstep; invc_vtm; auto.
+Qed.
+
+Lemma vtm_insert_address : forall m t1 t2 ad t T,
+  valid_term m t1 ->
+  t1 --[e_insert ad t T]--> t2 ->
+  ad < #m.
+Proof.
+  intros. ind_tstep; invc_vtm; auto.
+Qed.
+
+Lemma vtm_write_address : forall m t1 t2 ad t,
+  valid_term m t1 ->
+  t1 --[e_write ad t]--> t2 ->
+  ad < #m.
+Proof.
+  intros. ind_tstep; repeat invc_vtm; auto.
+Qed.
+
+(* lemmas about no-init and no-cr ------------------------------------------ *)
+
+(* spawn ------------------------ *)
+
+Lemma noinit_spawn_term : forall ad m t1 t2 tid t,
+  valid_term m t1 ->
+  t1 --[e_spawn tid t]--> t2 ->
+  no_init ad t.
+Proof.
+  intros. ind_tstep; invc_vtm; auto.
+Qed.
+
+Lemma nocr_spawn_term : forall ad m t1 t2 tid t,
+  valid_term m t1 ->
+  t1 --[e_spawn tid t]--> t2 ->
+  no_cr ad t.
+Proof.
+  intros. ind_tstep; invc_vtm; auto.
+Qed.
+
+Corollary noinits_spawn_term : forall m t1 t2 tid t,
+  valid_term m t1 ->
+  t1 --[e_spawn tid t]--> t2 ->
+  no_inits t.
+Proof.
+  unfold no_inits. eauto using noinit_spawn_term.
+Qed.
+
+Corollary nocrs_spawn_term : forall m t1 t2 tid t,
+  valid_term m t1 ->
+  t1 --[e_spawn tid t]--> t2 ->
+  no_crs t.
+Proof.
+  unfold no_crs. eauto using nocr_spawn_term.
+Qed.
+
+(* bounds ----------------------- *)
+
+Lemma noinit_from_vtm1 : forall m t,
+  valid_term m t ->
+  no_init (#m) t.
+Proof.
+  intros. induction t; invc_vtm; auto using no_init.
+Qed.
+
+Lemma noinit_from_vtm2 : forall ad m t,
+  valid_term m t ->
+  #m < ad ->
+  no_init ad t.
+Proof.
+  intros. induction t; invc_vtm; auto using no_init.
+  match goal with |- no_init ?ad1 <{init ?ad2 _ : _}> => nat_eq_dec ad1 ad2 end;
+  auto using no_init. lia.
+Qed.
+
+Lemma nocr_from_vtm1 : forall m t,
+  valid_term m t ->
+  no_cr (#m) t.
+Proof.
+  intros. induction t; invc_vtm; auto using no_cr.
+Qed.
+
+Lemma nocr_from_vtm2 : forall ad m t,
+  valid_term m t ->
+  #m < ad ->
+  no_cr ad t.
+Proof.
+  intros. induction t; invc_vtm; auto using no_cr.
+  match goal with |- no_cr ?ad1 <{cr ?ad2 _}> => nat_eq_dec ad1 ad2 end;
+  auto using no_cr. lia.
+Qed.
+
+(* values ----------------------- *)
+
+Lemma noinit_from_value : forall m ad t,
+  valid_term m t ->
+  (* --- *)
+  value t ->
+  no_init ad t.
+Proof.
+  intros * ? Hval. invc Hval; invc_vtm; auto using no_init.
+Qed.
+
+Lemma nocr_from_value : forall m ad t,
+  valid_term m t ->
+  (* --- *)
+  value t ->
+  no_cr ad t.
+Proof.
+  intros * ? Hval. invc Hval; invc_vtm; auto using no_cr.
+Qed.
+
+Corollary noinits_from_value : forall m t,
+  valid_term m t ->
+  (* --- *)
+  value t ->
+  no_inits t.
+Proof.
+  unfold no_inits. eauto using noinit_from_value.
+Qed.
+
+Corollary nocrs_from_value : forall m t,
+  valid_term m t ->
+  (* --- *)
+  value t ->
+  no_crs t.
+Proof.
+  unfold no_crs. eauto using nocr_from_value.
+Qed.
+
+(* preservation lemmas ----------------------------------------------------- *)
+
+Lemma vtm_subst : forall m t tx x,
+  no_inits t  ->
+  no_crs   t  ->
+  value    tx ->
+  (* --- *)
+  valid_term m t ->
+  valid_term m tx ->
+  valid_term m <{[x := tx] t}>.
+Proof.
+  intros. induction t; invc_noinits; invc_nocrs; invc_vtm;
+  simpl; try destruct _str_eq_dec; auto using valid_term;
+  constructor;
+  eauto using noinits_from_value, noinits_subst;
+  eauto using nocrs_from_value, nocrs_subst.
+Qed.
+
+Lemma vtm_mem_add : forall m t c,
+  valid_term m t ->
+  valid_term (m +++ c) t.
+Proof.
+  intros. induction t; invc_vtm; constructor; sigma; auto.
+Qed.
+
+Lemma vtm_mem_set : forall m t ad' t',
+  valid_term m t ->
+  valid_term m[ad'.t <- t'] t.
+Proof.
+  intros. induction t; invc_vtm; constructor; sigma; auto.
+Qed.
+
+Lemma vtm_mem_acq : forall m t ad,
+  valid_term m t ->
+  valid_term m[ad.X <- true] t.
+Proof.
+  intros. induction t; invc_vtm; constructor; sigma; auto.
+Qed.
+
+Lemma vtm_mem_rel : forall m t ad,
+  valid_term m t ->
+  valid_term m[ad.X <- false] t.
+Proof.
+  intros. induction t; invc_vtm; constructor; sigma; auto.
+Qed.
+
+Lemma vtm_mem_region : forall m t ad R,
+  valid_term m t ->
+  valid_term m[ad.R <- R] t.
+Proof.
+  intros. induction t; invc_vtm; constructor; sigma; auto.
+Qed.
+
+(* preservation ------------------------------------------------------------ *)
+
+Local Ltac solve_vtm_preservation :=
+  intros; ind_tstep; repeat invc_vtm; try constructor; sigma;
+  auto using vtm_subst, vtm_mem_add, vtm_mem_set, vtm_mem_acq, vtm_mem_rel.
+
+Lemma vtm_preservation_none : forall m t1 t2,
+  valid_term m t1 ->
+  t1 --[e_none]--> t2 ->
+  valid_term m t2.
+Proof. solve_vtm_preservation. Qed.
+
+Lemma vtm_preservation_alloc : forall m t1 t2 T,
+  valid_term m t1 ->
+  t1 --[e_alloc (#m) T]--> t2 ->
+  valid_term (m +++ (None, T, false, R_invalid)) t2.
+Proof. solve_vtm_preservation. Qed.
+
+Lemma vtm_preservation_insert : forall m t1 t2 ad t T,
+  valid_term m t1 ->
+  t1 --[e_insert ad t T]--> t2 ->
+  valid_term (m[ad.t <- t]) t2.
+Proof. solve_vtm_preservation. Qed.
+
+Lemma vtm_preservation_read : forall m t1 t2 ad t,
+  valid_term m t ->
+  (* --- *)
+  valid_term m t1 ->
+  t1 --[e_read ad t]--> t2 ->
+  valid_term m t2.
+Proof. solve_vtm_preservation. Qed.
+
+Lemma vtm_preservation_write : forall m t1 t2 ad t,
+  valid_term m t1 ->
+  t1 --[e_write ad t]--> t2 ->
+  valid_term (m[ad.t <- t]) t2.
+Proof. solve_vtm_preservation. Qed.
+
+Lemma vtm_preservation_acq : forall m t1 t2 ad t,
+  value t ->
+  valid_term m t ->
+  (* --- *)
+  valid_term m t1 ->
+  t1 --[e_acq ad t]--> t2 ->
+  valid_term m[ad.X <- true] t2.
+Proof. solve_vtm_preservation. Qed.
+
+Lemma vtm_preservation_rel : forall m t1 t2 ad,
+  valid_term m t1 ->
+  t1 --[e_rel ad]--> t2 ->
+  valid_term m[ad.X <- false] t2.
+Proof. solve_vtm_preservation. Qed.
+
+Lemma vtm_preservation_spawn : forall m t1 t2 tid t,
+  valid_term m t1 ->
+  t1 --[e_spawn tid t]--> t2 ->
+  valid_term m t2.
+Proof. solve_vtm_preservation. Qed.
+
+Lemma vtm_preservation_spawned : forall m t1 t2 tid t,
+  valid_term m t1 ->
+  t1 --[e_spawn tid t]--> t2 ->
+  valid_term m t.
+Proof. solve_vtm_preservation. Qed.
+
+(* ------------------------------------------------------------------------- *)
+
+Corollary vtm_preservation_memory : forall m1 m2 ths1 ths2 tid e,
+  forall_threads ths1 (valid_term m1) ->
+  forall_memory  m1   (valid_term m1) ->
+  m1 / ths1 ~~[tid, e]~~> m2 / ths2 ->
+  forall_memory  m2   (valid_term m2).
+Proof.
+  intros. invc_cstep; try invc_mstep; trivial; intros ? ? ?.
+  - upsilon. eauto using vtm_mem_add.
+  - upsilon; eauto using vtm_insert_term, vtm_mem_set.
+  - upsilon; eauto using vtm_write_term, vtm_mem_set.
+  - upsilon. eauto using vtm_mem_acq.
+  - upsilon. eauto using vtm_mem_rel.
+Qed.
+
+Corollary vtm_preservation_threads : forall m1 m2 ths1 ths2 tid e,
+  forall_memory  m1 value ->
+  (* --- *)
+  forall_memory  m1   (valid_term m1) ->
+  forall_threads ths1 (valid_term m1) ->
+  m1 / ths1 ~~[tid, e]~~> m2 / ths2 ->
+  forall_threads ths2 (valid_term m2).
+Proof.
+  intros. invc_cstep; try invc_mstep.
+  - upsilon. eauto using vtm_preservation_none.
+  - upsilon; eauto using vtm_mem_add, vtm_preservation_alloc.
+  - upsilon; eauto using vtm_mem_set, vtm_preservation_insert.
+  - upsilon. eauto using vtm_preservation_read.
+  - upsilon; eauto using vtm_mem_set, vtm_preservation_write.
+  - upsilon; eauto using vtm_mem_acq, vtm_preservation_acq.
+  - upsilon; eauto using vtm_mem_rel, vtm_preservation_rel.
+  - upsilon; eauto using vtm_preservation_spawn, vtm_preservation_spawned.
+Qed.
+
+Theorem vtm_preservation_cstep : forall m1 m2 ths1 ths2 tid e,
+  forall_memory  m1 value ->
+  (* --- *)
+  forall_program m1 ths1 (valid_term m1) ->
+  m1 / ths1 ~~[tid, e]~~> m2 / ths2 ->
+  forall_program m2 ths2 (valid_term m2).
+Proof.
+  intros * ? [? ?] ?. split;
+  eauto using vtm_preservation_memory, vtm_preservation_threads.
+Qed.
+
+Theorem vtm_preservation_rstep : forall m1 m2 ths1 ths2 tid e,
+  forall_memory  m1 value ->
+  (* --- *)
+  forall_program m1 ths1 (valid_term m1) ->
+  m1 / ths1 ~~~[tid, e]~~> m2 / ths2 ->
+  forall_program m2 ths2 (valid_term m2).
+Proof.
+  intros. invc_ostep; eauto using vtm_preservation_cstep.
+  match goal with _ : _ / _ ~~[_, _]~~> ?m / ?ths |- _ =>
+    assert (forall_program m ths (valid_term m)) as [? ?]
+      by eauto using vtm_preservation_cstep
+  end.
+  split; repeat intro; repeat omicron; upsilon; eauto using vtm_mem_region.
+Qed.
+
+Theorem vtm_preservation_ustep : forall m1 m2 ths1 ths2 tc,
+  forall_memory  m1 value ->
+  (* --- *)
+  forall_program m1 ths1 (valid_term m1) ->
+  m1 / ths1 ~~[tc]~~>* m2 / ths2 ->
+  forall_program m2 ths2 (valid_term m2).
+Proof.
+  intros. ind_ustep;
+  eauto using value_preservation_ustep, vtm_preservation_rstep.
+Qed.
+
+Theorem vtm_preservation_base : forall t,
+  no_refs  t ->
+  no_inits t ->
+  no_crs   t ->
+  (* --- *)
+  forall_program base_m (base_t t) (valid_term base_m).
+Proof.
+  auto using forall_program_base, vtm_from_base, valid_term.
+Qed.
+
