Values.v
@@ -25,12 +25,32 @@ Proof.
   intros * H. invc H; simpl; try destruct _str_eq_dec; auto using value.
 Qed.
 
-Theorem value_preservation : forall m1 m2 ths1 ths2 tid e,
+Theorem value_preservation_cstep : forall m1 m2 ths1 ths2 tid e,
   forall_memory m1 value ->
   m1 / ths1 ~~[tid, e]~~> m2 / ths2 ->
   forall_memory m2 value.
 Proof.
   intros. invc_cstep; trivial. invc_mstep; trivial;
   intros ? ? ?; upsilon; eauto using value_insert_term, value_write_term.
+Qed.
+
+Theorem value_preservation_rstep : forall m1 m2 ths1 ths2 tid e,
+  forall_memory m1 value ->
+  m1 / ths1 ~~~[tid, e]~~> m2 / ths2 ->
+  forall_memory m2 value.
+Proof.
+  intros. invc_ostep; eauto using value_preservation_cstep.
+  match goal with _ : _ / _ ~~[_, _]~~> ?m / ?ths |- _ =>
+    assert (forall_memory m value) by eauto using value_preservation_cstep
+  end.
+  repeat intro; repeat omicron; upsilon; eauto.
+Qed.
+
+Theorem value_preservation_ustep : forall m1 m2 ths1 ths2 tc,
+  forall_memory m1 value ->
+  m1 / ths1 ~~[tc]~~>* m2 / ths2 ->
+  forall_memory m2 value.
+Proof.
+  intros. ind_ustep; eauto using value_preservation_rstep.
 Qed.
 
